dw/DeepWeb/Proofs/TopLevelProof.v
@@ -1,0 +1,66 @@
+From DeepWeb.Spec
+     Require Import TopLevelSpec Swap_CLikeSpec
+     Vst.MainInit Vst.Gprog Vst.SocketSpecs.
+
+From DeepWeb.Proofs.Vst
+     Require Import verif_prog.
+  
+Theorem prog_correct: semax_prog_ext prog server Vprog Gprog.
+Proof.
+  unfold semax_prog_ext.
+
+  Print Ltac prove_semax_prog.
+  split3; [| | split3; [| | split ] ].
+  { auto. }
+  { reflexivity. }
+  { unfold cenv_cs, prog_comp_env.
+    unfold prog.
+    unfold CompSpecs.
+    match goal with
+    | |- ?LHS = _ =>
+      remember LHS as lhs
+    end.
+
+    unfold prog_comp_env.
+    unfold Clightdefs.mkprogram.
+    unfold build_composite_env'.
+    unfold build_composite_env.
+    simpl add_composite_definitions.
+    idtac.
+    simpl.
+    
+
+
+    
+    subst lhs.
+    f_equal.
+    repeat f_equal.
+    idtac.
+    apply proof_irr.
+    Set Printing All.
+l    
+    compute; repeat f_equal; apply proof_irr. 
+
+    unfold cenv_cs.
+    unfold prog_comp_env.
+    Print Ltac prove_semax_prog.
+    Print split3.
+    simpl.
+  } 
+    
+  split.
+  { admit. }
+  split. 
+  { apply all_funcs_correct. }
+  split.
+  { auto. }
+  admit.
+Admitted. 
+  
+
+Theorem swap_server_is_correct : swap_server_correct.
+Proof.
+  unfold swap_server_correct.
+  exists server.
+  apply prog_correct.
+Qed.
