dw/DeepWeb/Proofs/Vst/verif_accept_connection.v
@@ -1,0 +1,280 @@
+Require Import String.
+
+From DeepWeb.Spec.Vst
+     Require Import MainInit SocketSpecs Gprog MonadExports
+     Representation accept_connection_spec.
+
+From DeepWeb.Lib
+     Require Import VstLib.
+
+From DeepWeb.Proofs.Vst
+     Require Import VerifLib SocketTactics Connection.
+
+Import SockAPIPred.
+Import TracePred.
+
+Require Import DeepWeb.Spec.Swap_CLikeSpec.
+
+Set Bullet Behavior "Strict Subproofs".
+
+Open Scope list.
+Open Scope logic.
+
+Opaque bind.
+
+Set Bullet Behavior "Strict Subproofs".
+
+Lemma body_accept_connection:
+  semax_body Vprog Gprog f_accept_connection (accept_connection_spec unit).
+Proof.
+  start_function.
+  unfold accept_connection.
+
+  forward_accept fd.
+  { entailer!. }
+
+  Intro vret.
+  destruct vret as
+      [[accept_res st_post_accept] accept_ret].
+  simpl.
+  Intros.
+  
+  (* Get bounds on return value first *)
+  assert (-1 <= accept_ret < Int.max_signed).
+  {
+    match goal with
+    | [H: context[_ \/ accept_ret = NO] |- _] =>
+      destruct H
+        as [ [_ [accept_ret_geq accept_ret_lt] ] | accept_ret_eq]
+    end; unfold NO in *; rep_omega.
+  }     
+  
+  forward_if.
+  {
+    match goal with
+    | [H: context[_ \/ accept_ret = NO] |- _] =>
+      destruct H
+        as [ [_ [accept_ret_geq accept_ret_lt] ] | accept_ret_eq];
+        [rep_omega | ]
+    end.
+    
+    match goal with
+    | [H1: accept_ret = NO, H2: accept_ret = NO -> _ |- _] =>
+      destruct (H2 H1) as [accept_res_eq st_post_accept_eq]
+    end.
+
+    rewrite accept_res_eq.
+    take_branch2 1.
+    forward.
+
+    rewrite (trace_bind_ret (None : option connection)).
+    Exists (None : option (connection * sockfd * val)).
+    Exists st.
+    Exists NO.
+    unfold NO.
+
+    repeat apply andp_right; auto.
+    - apply prop_right; repeat split; auto.
+      intros; omega.
+    - cancel.
+  }
+
+  assert (accept_ret <> NO) by (unfold NO in *; omega).
+    
+  match goal with
+  | [H1: accept_ret <> NO, H2: accept_ret <> NO -> _ |- _] =>
+    destruct (H2 H1)
+      as [client_conn
+            [client_fd
+               [accept_res_eq
+                  [accept_ret_eq
+                     [lookup_client_fd
+                        st_post_accept_eq]]]]]
+  end.
+  
+  rewrite accept_res_eq.
+
+  forward_if.
+  {
+    take_branch2 1.
+    rewrite trace_bind_assoc.
+    
+    forward_shutdown client_fd.
+    { subst accept_ret; apply prop_right; repeat split; auto. }
+    { subst. repeat split; [assumption | | apply trace_incl_refl].
+      apply lookup_update_socket_eq; reflexivity.
+    }
+
+    Intro vret.
+    destruct vret as [st_post_shutdown shutdown_ret].
+    simpl.
+    Intros.
+
+    (* close *)
+    forward_call (st_post_shutdown, client_fd).
+    { apply prop_right; simpl; subst; reflexivity. }
+    
+    Intro vret.
+    destruct vret as [st_post_close close_ret].
+    simpl.
+
+    Intros.
+    to_equal.
+    forward.
+    from_equal.
+    
+    Exists (None : option (connection * sockfd * val)).
+    Exists st_post_close.
+    Exists NO.
+    unfold NO.
+
+    assert (st_post_close = st).
+    { prove_socket_map_eq st client_fd. }
+
+    rewrite (trace_bind_ret (None : option connection)).
+    entailer!.
+  } 
+    
+  (* alloc connection *)
+  forward_call tt.
+
+  Intro vret.
+  destruct vret
+    as [conn_opt alloc_ret].
+  simpl.
+
+  Intros.
+  forward_if.
+  { (* precondition *)
+    apply denote_tc_test_eq_split; [| apply valid_pointer_zero].
+    match goal with
+    | [H1: isptr alloc_ret \/ _,
+       H2: isptr alloc_ret -> _,
+       H3: alloc_ret = nullval -> _  |- _] =>
+      destruct H1 as [alloc_ret_ptr | alloc_ret_null];
+        [rewrite (H2 alloc_ret_ptr) | rewrite (H3 alloc_ret_null)]
+    end.
+
+    - entailer!.
+    - entailer!.
+  } 
+  
+  { (* if *)
+    match goal with
+    | [H1: alloc_ret = nullval,
+       H2: alloc_ret = nullval -> _ |- _] =>
+      rewrite (H2 H1)
+    end.
+    
+    take_branch2 2.
+    rewrite trace_bind_assoc.
+    forward_shutdown client_fd.
+    { subst accept_ret; apply prop_right; reflexivity. }
+    { repeat split;
+        [assumption | | apply trace_incl_refl ];
+        subst; apply lookup_update_socket_eq;
+        reflexivity. }
+
+    Intro vret.
+    destruct vret as [st_post_shutdown shutdown_ret].
+    simpl.
+    Intros.
+
+    (* close *)
+    forward_call (st_post_shutdown, client_fd).
+    { apply prop_right; simpl; subst; reflexivity. }
+
+    Intro vret.
+    destruct vret as [st_post_close close_ret].
+    simpl.
+    Intros.
+
+    trace_bind_ret.
+
+    assert (st_post_close = st).
+    { prove_socket_map_eq st client_fd. }
+
+    to_equal.
+    forward.
+    from_equal.
+    
+    Exists (None : option (connection * sockfd * val)).
+    Exists st_post_close.
+    Exists NO.
+    unfold NO.
+
+    repeat apply andp_right; auto.
+    - apply prop_right; repeat split; auto.
+      intros Hcontra; omega.
+    - subst.
+      cancel.
+  }
+
+  match goal with
+  | [H1: isptr alloc_ret \/ _,
+     H2: isptr alloc_ret -> _,
+     H3: alloc_ret = nullval -> _  |- _] =>
+    destruct H1 as [alloc_ret_ptr | alloc_ret_null];
+      [pose proof (H2 alloc_ret_ptr) as conn_opt_eq; rewrite conn_opt_eq
+      | tauto];
+      clear H1 H2 H3
+  end.
+
+  Intros tail.
+  
+  match goal with
+  | [H: conn_opt = Some ?cn |- _] =>
+    remember cn as conn0
+  end.
+
+  take_branch1 6.
+  trace_bind_ret.
+
+  assert_PROP (field_compatible (Tstruct _connection noattr) [] alloc_ret)
+    by entailer!.
+  
+  forward_call (conn0, 
+                {| descriptor := 0; is_descriptor := zero_is_fd |},
+                client_fd,
+                alloc_ret).
+  { subst; apply prop_right; repeat split; auto. }
+
+  forward.
+  forward.
+  forward.
+
+  to_equal.
+  forward.
+  from_equal.
+  
+  set (conn := {| conn_id := client_conn;
+                  conn_request := "";
+                  conn_response := "";
+                  conn_response_bytes_sent := 0;
+                  conn_state := RECVING
+               |}).
+  
+  Exists (Some (conn, client_fd, alloc_ret)).
+  Exists st_post_accept.
+  Exists YES.
+  unfold YES, NO.
+
+  repeat apply andp_right; auto.
+  { 
+    apply prop_right; repeat split; [omega | | omega | omega | assumption].
+    intros _.
+    exists client_conn; exists client_fd; exists alloc_ret.
+    repeat split; auto.
+    unfold FD_SETSIZE.
+    rewrite <- accept_ret_eq.
+    trivial.
+  }
+
+  cancel.
+
+  unfold rep_connection.
+  autounfold with updates; simpl.
+  Exists curr_head.
+  entailer!.
+  
+Qed.
