dw/DeepWeb/Proofs/Vst/verif_bind_socket.v
@@ -1,0 +1,85 @@
+From Custom Require Import String.
+
+From DeepWeb.Spec.Vst
+     Require Import MainInit Gprog SocketSpecs bind_socket_spec.
+
+From DeepWeb.Lib
+     Require Import VstLib.
+
+From DeepWeb.Proofs.Vst
+     Require Import VerifLib.
+
+Import SockAPIPred.
+Import SockAddr.
+
+Lemma body_bind_socket:
+  semax_body Vprog Gprog f_bind_socket bind_socket_spec.
+Proof.
+  start_function.
+
+  forward_call v_addr.
+  unfold_data_at 1%nat.
+  simpl.
+
+  forward.
+  forward.
+
+  assert
+    (Int.zero_ext 16 (Int.repr (port_number addr)) = Int.repr (port_number addr))
+    as addr_eq.
+  { rewrite zero_ext_inrange; [reflexivity |].
+    rewrite Int.unsigned_repr.
+    2: {
+      unfold Int.max_unsigned, two_p, two_power_pos in *.
+      simpl in *.
+      rep_omega.
+    }
+    omega.
+  } 
+  
+  forward_call (port_number addr).
+  { rewrite addr_eq. entailer!. }
+
+  forward.
+
+  forward_call (st, fd, addr, v_addr, sizeof (Tstruct _sockaddr_in noattr)).
+  { 
+    unfold_data_at 1%nat.
+    rewrite addr_eq.
+    cancel.
+  } 
+
+  Intro vret.
+  destruct vret as [st' bind_ret].
+  simpl.
+  Intros.
+
+  unfold YES, NO in *.
+
+  forward_if.
+  {
+    assert (bind_ret = -1) by omega.
+    match goal with
+    | [H1: bind_ret = -1, H2 : bind_ret = -1 -> _ |- _] =>
+      rewrite (H2 H1)
+    end.
+    forward.
+    Exists st.
+    Exists (-1).
+    entailer!.
+
+  }
+
+  assert (bind_ret = 0) by omega.
+  match goal with
+  | [H1: bind_ret = 0, H2 : bind_ret = 0 -> _ |- _] =>
+    destruct (H2 H1)
+      as [lookup_fd st'_eq]
+  end.
+
+  forward.
+  Exists (update_socket_state st fd (BoundSocket addr)).
+  Exists 0.
+  entailer!.
+
+Qed.
