dw/DeepWeb/Proofs/Vst/verif_check_if_complete.v
@@ -1,0 +1,48 @@
+Require Import String.
+
+Require Import DeepWeb.Spec.Swap_CLikeSpec.
+
+From DeepWeb.Spec.Vst
+     Require Import MainInit Gprog check_if_complete_spec.
+
+From DeepWeb.Lib
+     Require Import VstLib.
+
+From DeepWeb.Proofs.Vst
+     Require Import VerifLib.
+
+Set Bullet Behavior "Strict Subproofs".
+
+Lemma body_check_if_complete:
+  semax_body Vprog Gprog f_check_if_complete
+             (check_if_complete_spec BUFFER_SIZE).
+Proof.
+  start_function.
+
+  forward_if.
+  {
+    forward.
+    Exists 1.
+    entailer!.
+
+    unfold is_complete.
+    rewrite Z.eqb_eq.
+    autorewrite_sublist.
+    unfold BUFFER_SIZE.
+    assumption.
+  } 
+
+  forward.
+
+  Exists 0.
+  entailer!.
+  unfold is_complete.
+  rewrite <- not_true_iff_false.
+  unfold not, BUFFER_SIZE; intros Hsize.
+  apply H0.
+  revert Hsize.
+  autorewrite_sublist.
+  rewrite Z.eqb_eq.
+  intros; auto.
+  
+Qed.  
