dw/DeepWeb/Proofs/Vst/verif_conn_read.v
@@ -1,0 +1,464 @@
+Require Import String.
+
+Require Import DeepWeb.Spec.Swap_CLikeSpec.
+
+From DeepWeb.Spec.Vst
+     Require Import MainInit Gprog SocketSpecs MonadExports
+     Representation AppLogic conn_read_spec.
+
+From DeepWeb.Lib
+     Require Import VstLib.
+
+From DeepWeb.Proofs.Vst
+     Require Import VerifLib SocketTactics Connection.
+
+Import SockAPIPred.
+Import TracePred.
+
+Open Scope list.
+Open Scope logic.
+
+Opaque bind.
+
+Set Bullet Behavior "Strict Subproofs".
+
+Lemma body_conn_read:
+  semax_body Vprog Gprog f_conn_read (conn_read_spec unit BUFFER_SIZE).
+Proof.
+  start_function.
+
+  assert_PROP (field_compatible (Tstruct _connection noattr)
+                                [] (conn_ptr))
+    by entailer!.
+  
+  assert_PROP
+    (field_compatible (Tstruct _connection noattr)
+                      [StructField _request_buffer] (conn_ptr))
+    by entailer!.
+
+  match goal with
+  | [H: context[consistent_state] |- _] =>
+    inversion H; subst; try discriminate
+  end.
+
+  match goal with
+  | [H: consistent_state _ _ (?c, _) |- _] =>
+    set (conn := c)
+  end.
+
+  unfold rep_connection.
+  rewrite connection_list_cell_eq; [| assumption].                                        
+  Intros.
+
+  do 4 forward.
+  
+  freeze [2; 3; 5; 6; 7; 8; 9] FR1.
+  simpl.
+
+  (* recv *)
+  
+  (* Split at current end of msg to recv there *)
+  focus_SEP 3.
+  rewrite field_at_data_at.
+  simpl.
+  saturate_rep_msg_bounds.
+  
+  split_data_at (Zlength (val_of_string (conn_request conn))).
+  2 : { simpl; omega. }
+  Intros.
+  
+  freeze [0] FR2.
+  focus_SEP 1.
+  rem_ptr buf_ptr.
+    
+  unfold conn_read.
+
+  replace (BUFFER_SIZE - Z.of_nat (String.length (conn_request conn)))
+    with (1024 - Zlength (val_of_string (conn_request conn))).
+  2 : {
+    unfold BUFFER_SIZE.
+    autorewrite_sublist.
+    reflexivity.
+  }
+  
+  forward_recv fd buf_ptr
+  (1024 - Zlength (val_of_string (conn_request conn))).
+  { (* buffer pointer equality *)
+    apply prop_right; repeat split; auto.
+    subst; simpl.
+    unfold rep_msg_len.
+    rewrite sem_add_pi_ptr_special.
+    2 : {
+      apply isptr_offset_val'.
+      auto.
+    }
+    rewrite field_address0_offset.
+    2 : {
+      prove_field_compatible0_array_field_addr.
+      rewrite field_address_offset; auto.
+    }
+
+    simpl.
+    rewrite field_address_offset; auto.
+  } 
+  { (* trace *) subst; cancel. }
+
+  Intro vret.
+  destruct vret as [[[recv_res st_post_recv] recv_ret] contents].
+
+  simpl fst; simpl snd.
+  Intros.
+
+  (* Derive basic bounds on return value *)
+  assert (-1 <= recv_ret < Int.max_signed).
+  { match goal with
+    | [H: _ \/ recv_ret = NO |- _] =>
+      unfold NO in H; destruct H; try rep_omega
+    end.
+  } 
+
+  (* Coalesce buffer first *)
+  thaw FR2.
+  gather_SEP 3 2.
+  subst buf_ptr.
+  coalesce.
+  
+  forward_if.
+  {
+
+    match goal with
+    | [H1 : recv_ret < 0, H2 : recv_ret < 0 -> _ |- _] =>
+      destruct (H2 H1)
+        as [recv_res_eq [contents_eq st_post_recv_eq]]
+    end.
+
+    subst recv_res.
+
+    take_branch2 2.
+    trace_bind_ret.
+    subst contents.
+    fold_rep_msg.
+
+    thaw FR1; simpl.
+    Intros.
+
+    to_equal.
+    forward.
+    from_equal.
+    
+    Exists conn.
+    Exists last_msg.
+    Exists st.
+    Exists YES.
+
+    repeat apply andp_right; auto.
+    { apply prop_right; repeat split; auto.
+      apply Conn_RECVING_Id.
+    } 
+
+    unfold rep_connection.
+    rewrite connection_list_cell_eq; [| assumption].
+    unfold BUFFER_SIZE.
+    cancel.
+    rewrite field_at_data_at; simpl; subst; cancel.
+
+  }
+
+  forward_if.
+  { (* EOF *)
+    
+
+    match goal with
+    | [H1 : recv_ret = 0, H2 : recv_ret = 0 -> _ |- _] =>
+      destruct (H2 H1)
+        as [recv_res_eq [contents_eq st_post_recv_eq]]
+    end.
+    subst recv_res.
+    trace_bind_ret.
+    
+    subst contents.
+    fold_rep_msg.
+    
+    thaw FR1.
+    simpl.
+    Intros.
+
+    forward.
+    
+    to_equal.
+    forward.
+    from_equal.
+
+    Exists (upd_conn_state conn DELETED).
+    Exists last_msg.
+    Exists (update_socket_state st fd OpenedSocket).
+    Exists YES.
+    
+    repeat apply andp_right; auto.
+    { apply prop_right; repeat split; auto.
+      - apply Conn_RECVING_EOF; subst; auto.
+      - subst; assumption.
+    }       
+
+    unfold rep_connection.
+    rewrite connection_list_cell_eq; [| assumption].
+    unfold BUFFER_SIZE.
+    rewrite field_at_data_at; simpl; cancel.
+    autounfold with updates.
+    rewrite field_at_data_at.
+    subst.
+    cancel.
+    
+    
+  } 
+
+  assert (recv_ret > 0) by omega.
+  match goal with
+  | [H1 : recv_ret > 0, H2 : recv_ret > 0 -> _ |- _] =>
+    destruct (H2 H1)
+      as [[msg [recv_res_eq
+                  [msg_len_eq
+                     [contents_prefix contents_suffix]]]] st_post_recv_eq]
+  end.
+  subst recv_res.
+
+  match goal with
+  | [H: _ \/ recv_ret = NO |- _] =>
+    destruct H as [recv_ret_bounds | recv_ret_eq];
+      [| unfold NO in recv_ret_eq; subst recv_ret; omega ]
+  end.
+
+  (* Coalesce with new msg *)
+  match goal with
+  | [H1: sublist 0 _ _ = ?prefix, H2: sublist recv_ret _ _ = ?suffix |- _] =>
+    assert (contents = (prefix ++ suffix))
+  end.
+  { 
+    rewrite <- contents_prefix.
+    rewrite <- contents_suffix.
+    rewrite <- sublist_split; [ | omega | split; omega].
+    rewrite sublist_same; auto.
+  }
+  
+  subst contents.
+  rewrite List.app_assoc.
+  rewrite <- val_of_string_app.
+  subst recv_ret.
+  fold_rep_msg.
+  2: { simpl in *|- ; omega. }
+
+  match goal with
+  | [|- context[data_at _ _ (rep_msg _ ?bound) _]] =>
+    replace bound with 1024
+  end.
+  2 : {
+    rewrite <- Z.sub_add_distr.
+    autorewrite_sublist.
+    reflexivity.
+  } 
+  
+  (* End Coalesce *)
+  
+  thaw FR1.
+  simpl.
+
+  forward.
+  forward.
+
+  (* is_complete *)
+
+  freeze [1; 2; 3; 4; 5; 6; 7; 8] FR1.
+  simpl.
+  
+  (* Split again for check *)
+  focus_SEP 1.
+  saturate_rep_msg_bounds.
+  unfold rep_msg.
+
+  split_data_at.
+  Intros.
+
+  forward_call ((conn_request conn ++ msg)%string,
+                field_address (Tstruct _connection noattr)
+                              [StructField _request_buffer] conn_ptr,
+                Zlength (val_of_string (conn_request conn ++ msg)),
+                Tsh).
+  { entailer!.
+    autorewrite_sublist.
+    split; auto.
+    rewrite field_address_offset by assumption.
+    auto.
+  }
+
+  {
+    split; auto.
+    subst conn; simpl.
+    rep_omega.
+  } 
+
+  Intro is_complete_ret.
+  Intros.
+
+  (* Coalesce again *)
+  gather_SEP 0 1.
+  coalesce.
+  fold_rep_msg.
+  thaw FR1.
+  simpl.
+
+  (*
+  replace (Zlength _ >? _) with false.
+
+  2 : {
+    unfold BUFFER_SIZE in *.
+    
+    symmetry.
+    rewrite <- not_true_iff_false.
+    unfold not.
+    intros Hcontra.
+    rewrite <- Zgt_is_gt_bool in Hcontra.
+
+    match goal with
+    | [H: Zlength (val_of_string _) <= _ |- _] =>
+      revert H
+    end.
+    
+    rewrite val_of_string_app.
+    rewrite Zlength_app.
+    intros.
+    omega.
+
+  } 
+  *)
+  
+  forward_if.
+  {
+    (* Have more to receive *)
+    
+    match goal with
+    | [H1: is_complete_ret = 0, H2: is_complete_ret = 0 -> _ |- _] =>
+      simpl conn_request in H2; rewrite (H2 H1)
+    end.
+
+    set (conn' := {| conn_id := conn_id conn;
+                     conn_request := conn_request conn ++ msg;
+                     conn_response := conn_response conn;
+                     conn_response_bytes_sent := conn_response_bytes_sent conn;
+                     conn_state := RECVING
+                  |}).
+    trace_bind_ret.
+
+    to_equal.
+    forward.
+    from_equal.
+
+    Exists conn'.
+    Exists last_msg.
+    Exists st_post_recv.
+    Exists YES.
+
+    subst conn' st_post_recv.
+    
+    repeat apply andp_right; auto.
+    { apply prop_right; repeat split; auto.
+      eapply Conn_RECVING_RECVING; subst; simpl; auto.
+    } 
+
+    unfold rep_connection.
+    rewrite connection_list_cell_eq; [| assumption].
+    simpl.
+    repeat rewrite field_at_data_at; simpl.
+    cancel.
+    autorewrite_sublist.
+    cancel.
+  }
+
+  match goal with
+  | [H: is_complete_ret = _ \/ _ |- _] =>
+    destruct H; [| tauto ]
+  end.
+  
+  match goal with
+    | [H1: is_complete_ret = 1, H2: is_complete_ret = 1 -> _ |- _] =>
+      simpl in H2; rewrite (H2 H1)
+  end.
+  
+  forward.
+
+  (* populate response *)
+  data_at_to_field_at.
+
+  field_at_rebase_ptr.
+  
+  gather_SEP 3 4 0 5 6 7 8.
+  repeat rewrite <- sepcon_assoc.
+  rewrite <- connection_list_cell_eq; [| assumption].
+
+  set (conn_before_populate :=
+         {| conn_id := conn_id conn;
+            conn_request := conn_request conn ++ msg;
+            conn_response := conn_response conn;
+            conn_response_bytes_sent := conn_response_bytes_sent conn;
+            conn_state := conn_state conn
+         |}).            
+  
+  fold_rep_connection conn_before_populate fd.
+  {
+    go_lower.
+    rewrite add_repr.
+    subst conn_before_populate;
+    unfold rep_connection, BUFFER_SIZE;
+    simpl.
+    unfold rep_msg_len.
+    autorewrite_sublist.
+    cancel.
+  } 
+
+  forward_call (conn_before_populate,
+                fd,
+                last_msg,
+                conn_ptr,
+                msg_store_ptr).
+  
+  Intro vret.
+  destruct vret as [[populate_ret conn_post_populate] last_msg'].
+  simpl fst; simpl snd.
+  Intros.
+  
+  forward_if.
+  { (* impossible branch *)
+    omega.
+  } 
+  
+  unfold rep_connection.
+  rewrite connection_list_cell_eq; [| assumption].
+
+  Intros.
+  forward.
+
+  gather_SEP 0 1 2 3 4 5 6 7 8.
+  repeat rewrite <- sepcon_assoc.
+  rewrite <- connection_list_cell_eq; [| assumption].
+  
+  trace_bind_ret.
+  
+  to_equal.
+  forward.
+  from_equal.
+
+  Exists (upd_conn_state conn_post_populate SENDING).
+  Exists last_msg'.
+  Exists st_post_recv.
+  Exists YES.
+
+  subst conn_post_populate conn_before_populate st_post_recv last_msg'.
+  repeat apply andp_right; auto.
+  - apply prop_right; repeat split; auto.
+    apply Conn_RECVING_SENDING; subst; simpl; auto.
+  - autounfold with updates.
+    simpl.
+    unfold rep_connection, rep_connection_state.
+    simpl.
+    cancel.
+      
+Qed.
