dw/DeepWeb/Proofs/Vst/verif_conn_write.v
@@ -1,0 +1,339 @@
+Require Import String.
+
+Require Import DeepWeb.Spec.Swap_CLikeSpec.
+
+From DeepWeb.Spec.Vst
+     Require Import MainInit Gprog SocketSpecs MonadExports
+     AppLogic Representation conn_write_spec.
+
+From DeepWeb.Lib
+     Require Import VstLib.
+
+From DeepWeb.Proofs.Vst
+     Require Import VerifLib SocketTactics Connection.
+
+Import SockAPIPred.
+Import TracePred.
+
+Open Scope list.
+Open Scope logic.
+
+Opaque bind.
+
+Set Bullet Behavior "Strict Subproofs".
+
+
+Lemma body_conn_write:
+  semax_body Vprog Gprog f_conn_write (conn_write_spec unit BUFFER_SIZE).
+Proof.
+  start_function.
+
+  assert_PROP (field_compatible (Tstruct _connection noattr)
+                                [] (conn_ptr))
+    by entailer!.
+
+  assert_PROP (field_compatible (Tstruct _connection noattr)
+                                [StructField _response_buffer] conn_ptr)
+    by entailer!.
+
+  match goal with
+  | [H: consistent_state _ _ _ |- _] =>
+    inversion H; subst; try discriminate
+  end.
+  
+  match goal with
+  | [H: consistent_state _ _ (?c, _) |- _] =>
+    set (conn := c)
+  end.
+
+  unfold rep_connection.
+  rewrite connection_list_cell_eq; [| auto].
+  
+  Intros.
+  do 5 forward.
+
+  match goal with
+  | [|- context[ITREE _]] =>
+  match goal with
+  | [|- context[SOCKAPI _]] =>
+  match goal with
+  | [|- context[field_at _ _ [StructField _response_buffer] _ _]] =>
+    freeze [2; 3; 4; 5; 7; 8] FR1; simpl
+  end
+  end
+  end.
+
+  focus_SEP 3.
+  rewrite field_at_data_at; simpl.
+  saturate_rep_msg_bounds.
+  unfold rep_msg.
+  split_data_at. (* first split from undefined tail *)
+  Intros.
+
+  freeze [1; 2] FR2; simpl.
+  focus_SEP 1.
+  
+  (* then split from what's been sent *)
+  split_data_at (conn_response_bytes_sent conn).
+  2: {
+    subst conn; auto.
+  } 
+  Intros.
+  freeze [0; 2] FR3; simpl.
+
+  focus_SEP 1.
+  rem_ptr buf_ptr.
+  unfold conn_write.
+  
+  forward_send fd buf_ptr.
+  { apply prop_right; repeat split; auto.
+    - (* Unifying pointers *)
+      simpl.
+      rewrite sem_add_pi_ptr_special.
+      2 : {
+        apply isptr_offset_val'.
+        auto.
+      }
+      subst; simpl.
+      rewrite field_address0_offset; simpl.
+      2 : {
+        prove_field_compatible0_array_field_addr.
+        simpl in Hcompat.
+        prove_field_compatible_smaller_array.
+        unfold tarray in Hcompat.
+        - rewrite field_address_offset; auto.
+        - unfold BUFFER_SIZE in *.
+          simpl in *|-.
+          auto.
+      } 
+      rewrite field_address_offset; auto.
+    - (* Unifying string length from ITree with Zlength in VST *)
+      simpl.
+      repeat f_equal.
+      repeat autorewrite_sublist; omega.
+  }
+  { cancel.
+    autorewrite_sublist;
+      [| autorewrite_sublist; subst; simpl; omega..].
+    cancel.
+  } 
+
+  Intro vret.
+  destruct vret as [[send_res st_post_send] send_ret].
+  simpl fst; simpl snd.
+
+  (* Rejoin buffer *)
+  Intros.
+  thaw FR3; thaw FR2; simpl.
+  rem_trace tr.
+  gather_SEP 2 3 4.
+  Intros.
+  subst buf_ptr.
+  gather_SEP 1 0.
+  autorewrite_sublist;
+    [| autorewrite_sublist; subst; simpl; omega..].
+  
+  Intros.
+  gather_SEP 0 1.
+  coalesce.
+  { autorewrite_sublist; omega. }
+  simpl.
+  rewrite sublist_firstn.
+  rewrite firstn_skipn.
+
+  gather_SEP 0 1.
+  coalesce.
+  fold_rep_msg.
+
+  (* Restore all fields *)
+  data_at_to_field_at.
+  field_at_rebase_ptr.
+  
+  thaw FR1; simpl.
+
+  assert (-1 <= send_ret < Int.max_signed).
+  {
+    match goal with
+    | [H: _ \/ send_ret = _ |- _] =>
+      unfold NO in H;
+        destruct H as [[send_ret_lb send_ret_ub] | ?];
+        try rep_omega
+    end.
+    subst; simpl in send_ret_ub. 
+    autorewrite_sublist in send_ret_ub;
+      [| autorewrite_sublist; omega..].
+    rep_omega.
+  } 
+
+  forward_if.
+  { (* send fails *)
+
+    subst tr.
+    assert (send_ret = NO) by (unfold NO; omega).
+    match goal with
+    | [H1: send_ret = NO, H2 : send_ret = NO -> _ |- _] =>
+      destruct (H2 H1) as [send_res_eq st_post_send_cases]
+    end.
+
+    subst send_res.
+    take_branch2 2.
+    trace_bind_ret.
+
+    forward.
+
+    forward.
+
+    Exists (upd_conn_state conn DELETED).
+    Exists st_post_send.
+    Exists YES.
+    repeat apply andp_right; auto.
+    - apply prop_right; repeat split; auto.
+      subst.
+      apply Conn_SENDING_Fail; auto.
+    - unfold rep_connection.
+      rewrite connection_list_cell_eq; [| assumption].
+      cancel.
+  }
+
+  forward.
+  
+  forward_if.
+  { (* send incomplete *)
+
+    subst tr.
+    assert (send_ret <> NO) by (unfold NO; omega).
+    match goal with
+    | [H1: send_ret <> NO, H2 : send_ret <> NO -> _ |- _] =>
+      destruct (H2 H1) as [send_res_eq st_post_send_eq]
+    end.
+
+    subst send_res.
+    assert ((String.length response <? Z.to_nat send_ret)%nat = false)
+      as dead_cond.
+    {
+      rewrite Nat.ltb_ge.
+      autorewrite_sublist.
+      omega.
+    }
+    
+    rewrite dead_cond.
+
+    autorewrite_sublist.
+    assert (num_bytes_sent + send_ret
+            =? Zlength (val_of_string response) = false)
+      as incomplete_cond.
+    { rewrite Z.eqb_neq.
+      unfold not; intros.
+      omega.
+    } 
+    rewrite incomplete_cond.
+
+    trace_bind_ret.
+
+    forward.
+
+    Exists ({| conn_id := client_id;
+               conn_request := request;
+               conn_response := response;
+               conn_response_bytes_sent := num_bytes_sent + send_ret;
+               conn_state := SENDING |}).
+    Exists st.
+    Exists YES.
+    unfold rep_connection.
+    rewrite connection_list_cell_eq; [| assumption].
+    simpl.
+    entailer!.
+    
+    apply Conn_SENDING_SENDING with (num_bytes_sent := send_ret);
+      simpl; auto; omega.
+
+    
+  }
+
+  subst tr.
+  assert (send_ret <> NO) by (unfold NO; omega).
+  match goal with
+  | [H1: send_ret <> NO, H2 : send_ret <> NO -> _ |- _] =>
+    destruct (H2 H1) as [send_res_eq st_post_send_eq]
+  end.
+
+  subst send_res.
+
+  match goal with
+  | [H: _ \/ send_ret = NO |- _] =>
+    destruct H as [[send_ret_lb send_ret_ub] | ?]; try rep_omega
+  end.
+
+  autorewrite_sublist in send_ret_ub;
+    [| autorewrite_sublist; omega ..].
+  
+  assert ((String.length response <? Z.to_nat send_ret)%nat = false)
+    as dead_cond.
+  {
+    rewrite Nat.ltb_ge.
+    autorewrite_sublist.
+    subst conn; simpl in send_ret_ub.
+    omega.
+  }
+
+  rewrite dead_cond.
+
+  autorewrite_sublist.
+  assert (num_bytes_sent + send_ret
+          =? Zlength (val_of_string response) = true)
+    as complete_cond.
+  { rewrite Z.eqb_eq.
+    subst conn; simpl in send_ret_ub.
+    omega.
+  } 
+
+  rewrite complete_cond.
+  trace_bind_ret.
+
+  gather_SEP 3 4 5 6 0.
+  Intros.
+  gather_SEP 0 1 2 3 4 7 8.
+  repeat rewrite <- sepcon_assoc.
+  rewrite <- connection_list_cell_eq by assumption.
+  
+  set (conn_pre_reset :=
+         {| conn_id := client_id;
+            conn_request := request;
+            conn_response := response;
+            conn_response_bytes_sent := num_bytes_sent + send_ret;
+            conn_state := SENDING
+         |}
+      ).
+
+  fold_rep_connection conn_pre_reset fd.
+  { go_lower. unfold rep_connection.
+    subst conn_pre_reset.
+    simpl.
+    rewrite add_repr.
+    cancel.
+  }
+
+  forward_call (conn_pre_reset, fd, fd, conn_ptr).
+  subst st_post_send.
+  
+  forward.
+
+  Exists ({| conn_id := client_id;
+             conn_request := "";
+             conn_response := "";
+             conn_response_bytes_sent := 0;
+             conn_state := RECVING |}).
+  Exists st.
+  Exists YES.
+  entailer!.
+  - apply Conn_SENDING_RECVING
+      with (num_bytes_sent :=
+              Zlength (val_of_string response) - num_bytes_sent);
+      [auto | | reflexivity | auto].
+    simpl.
+    omega.
+  - autounfold with updates.
+    simpl.
+    cancel.
+    
+Qed.
