dw/DeepWeb/Proofs/Vst/verif_init_store.v
@@ -1,0 +1,89 @@
+From Custom Require Import String.
+
+Require Import DeepWeb.Spec.ServerDefs.
+
+From DeepWeb.Spec.Vst
+     Require Import MainInit Gprog Representation init_store_spec.
+
+From DeepWeb.Lib
+     Require Import VstLib.
+
+From DeepWeb.Proofs.Vst
+     Require Import VerifLib Store.
+
+Set Bullet Behavior "Strict Subproofs".
+
+Lemma body_init_store:
+  semax_body Vprog Gprog f_init_store init_store_spec.
+Proof.
+  start_function.
+
+  forward.
+  forward.
+
+  unfold_field_at 1%nat.
+  focus_SEP 1.
+
+  assert_PROP (field_compatible (Tstruct _store noattr)
+                                [StructField _stored_msg_len] ptr)
+    by entailer!.
+  
+  assert_PROP (field_compatible (Tstruct _store noattr)
+                                [StructField _stored_msg] ptr)
+    by entailer!.
+
+  forward_call (field_address (Tstruct _store noattr)
+                              [StructField _stored_msg] ptr,
+                48, (* '0' *)
+                1024).
+  { 
+    entailer!.
+    rewrite field_address_offset by assumption.
+    simpl.
+    reflexivity.
+  } 
+  
+  { replace (1024 >? 0) with true
+      by (symmetry; rewrite <- Zgt_is_gt_bool; omega).
+    repeat rewrite field_at_data_at.
+    cancel.
+  }
+  { rep_omega. }
+
+  replace (1024 >? 0) with true
+    by (symmetry; rewrite <- Zgt_is_gt_bool; omega).
+
+  replace (list_repeat _ _) with (rep_msg INIT_MSG BUFFER_SIZE).
+  2 : {
+    unfold rep_msg.
+    assert (Zlength (val_of_string INIT_MSG) = BUFFER_SIZE) as Hmsg.
+    { unfold INIT_MSG.
+      rewrite Zlength_val_string_len.
+      rewrite repeat_string_length.
+      autorewrite_sublist; auto.
+      unfold BUFFER_SIZE; omega.
+    } 
+    rewrite Hmsg.
+    replace (BUFFER_SIZE - BUFFER_SIZE) with 0 by omega.
+    simpl list_repeat at 1.
+    rewrite app_nil_r.
+    unfold INIT_MSG.
+    rewrite repeat_string_list_repeat.
+    unfold BUFFER_SIZE.
+    f_equal.
+  }
+
+  data_at_to_field_at.
+  field_at_rebase_ptr.
+  focus_SEP 1.
+  data_at_to_field_at.
+  field_at_rebase_ptr.
+  { cancel. }
+  simpl.
+
+  gather_SEP 0 1.
+  erewrite <- field_at_rep_store_eq by reflexivity.
+
+  forward.
+  
+Qed.
