dw/DeepWeb/Proofs/Vst/verif_new_connection.v
@@ -1,0 +1,102 @@
+Require Import String.
+
+Require Import DeepWeb.Spec.Swap_CLikeSpec.
+
+From DeepWeb.Spec.Vst
+     Require Import MainInit Gprog SocketSpecs Representation
+     new_connection_spec.
+
+From DeepWeb.Lib
+     Require Import VstLib.
+
+From DeepWeb.Proofs
+     Require Import VerifLib Connection.
+
+Set Bullet Behavior "Strict Subproofs".
+
+Lemma body_new_connection:
+  semax_body Vprog Gprog f_new_connection new_connection_spec.
+Proof.
+  start_function.
+  forward_call (Tstruct _connection noattr).
+  { repeat split; simpl; auto; rep_omega. }
+
+  Intro conn_ptr.
+
+  forward_if.
+  { destruct conn_ptr; try tauto.
+    - simpl in PNconn_ptr.
+      subst.
+      entailer.
+    - simpl.
+      entailer.
+  }
+  { subst.
+    simpl.
+    forward.
+    Exists (None : option connection).
+    Exists nullval.
+    entailer!.
+  }
+
+  match goal with
+    | [|- context[if ?cond then _ else _]] =>
+      destruct cond; [tauto | ]
+  end.
+
+  Intros.
+
+  focus_SEP 1.
+  data_at_to_field_at_default.
+
+  do 6 forward.
+
+  set (new_conn := {| conn_id := Connection 0%nat;
+                      conn_request := "";
+                      conn_response := "";
+                      conn_response_bytes_sent := 0;
+                      conn_state := RECVING
+                   |}).
+
+  set (new_fd := {| descriptor := 0; is_descriptor := zero_is_fd |}).
+
+  match goal with
+  | [|- context[field_at _ _ _ ?rep _]] =>
+    assert
+      (rep = 
+       (Vint (Int.repr (descriptor new_fd)),
+        (rep_msg_len (conn_request new_conn),
+         (rep_msg (conn_request new_conn) BUFFER_SIZE,
+          (rep_msg_len (conn_response new_conn),
+           (rep_msg (conn_response new_conn) BUFFER_SIZE,
+            (Vint (Int.repr (conn_response_bytes_sent new_conn)),
+             (rep_connection_state (conn_state new_conn),
+              Vint (Int.repr 0))))))))) as Hrep by reflexivity;
+      rewrite Hrep;
+      clear Hrep
+  end.
+
+  unfold_field_at 1%nat.
+
+  gather_SEP 0 1 2 3 4 5 6.
+  repeat rewrite <- sepcon_assoc.
+  assert_PROP (field_compatible (Tstruct _connection noattr) [] conn_ptr)
+    by entailer!.
+  rewrite <- connection_list_cell_eq; [| assumption].
+  
+  fold_rep_connection new_conn new_fd.
+  { go_lower; subst new_conn; unfold rep_connection; simpl; cancel. }
+
+  forward.
+  Exists (Some new_conn).
+  Exists conn_ptr.
+  Exists nullval.
+
+  repeat apply andp_right; auto.
+  - apply prop_right; repeat split; auto. intros; tauto. 
+  - cancel.
+    apply andp_right; [entailer | cancel].
+    subst new_fd.
+    entailer.
+    
+Qed.
