dw/DeepWeb/Proofs/Vst/verif_new_store.v
@@ -1,0 +1,101 @@
+Require Import String.
+
+From DeepWeb.Spec.Vst
+     Require Import MainInit Gprog
+     Representation new_store_spec.
+
+From DeepWeb.Lib
+     Require Import VstLib.
+
+From DeepWeb.Proofs.Vst
+     Require Import VerifLib Store.
+
+Set Bullet Behavior "Strict Subproofs".
+
+Lemma body_new_store:
+  semax_body Vprog Gprog f_new_store new_store_spec.
+Proof.
+  start_function.
+  
+  forward_call (Tstruct _store noattr).
+  { repeat split; simpl; auto; rep_omega. }
+
+  Intro new_ptr.
+  
+  forward_if.
+  { destruct new_ptr; try tauto.
+    - simpl in PNnew_ptr.
+      subst.
+      entailer.
+    - simpl.
+      entailer.
+  }
+  { subst.
+
+    destruct (eq_dec nullval nullval);
+      forward.
+
+    Exists (None : option store).
+    Exists nullval.
+    entailer!.
+  }
+
+  destruct (eq_dec new_ptr nullval); [ tauto |].
+  
+  assert_PROP (field_compatible (Tstruct _store noattr) [] new_ptr)
+    by entailer!.
+  assert_PROP (field_compatible (Tstruct _store noattr)
+                                [StructField _stored_msg] new_ptr)
+    by entailer!.
+
+  Intros.
+  focus_SEP 1.
+
+  (* Promote to field first *)
+  data_at_to_field_at_default.
+  
+  match goal with
+  | [|- context[default_val ?v]] =>
+    remember (default_val v) as protected
+  end.
+
+  do 2 forward.
+  simpl.
+  erewrite field_at_rep_store_eq by (subst; reflexivity).
+  Intros.
+  focus_SEP 1.
+  rewrite field_at_data_at.
+  rewrite <- Heqprotected.
+  erase_data.
+
+  forward_call (offset_val 4 new_ptr, 0, 1024). 
+  { replace (1024 >? 0) with true
+      by (symmetry; rewrite <- Zgt_is_gt_bool; omega).
+    rewrite field_address_offset by assumption.
+    simpl.
+    cancel.
+  }
+  { rep_omega. }
+
+  replace (1024 >? 0) with true
+    by (symmetry; rewrite <- Zgt_is_gt_bool; omega).
+
+  match goal with
+  | [|- context[list_repeat ?n ?v]] =>
+    remember (list_repeat n v) as protected'
+  end.
+
+  forward.
+
+  Exists (Some {| stored_msg := "" |}) new_ptr.
+  unfold rep_store.
+  erewrite field_at_rep_store_eq; [| reflexivity].
+  rewrite rep_empty_string.
+  unfold BUFFER_SIZE.
+  repeat rewrite field_at_data_at.
+
+  entailer!.
+  rewrite field_address_offset by assumption.
+  cancel.
+
+Qed.
