dw/DeepWeb/Proofs/Vst/verif_process.v
@@ -1,0 +1,147 @@
+Require Import String.
+
+Require Import DeepWeb.Spec.Swap_CLikeSpec.
+
+From DeepWeb.Spec.Vst
+     Require Import MainInit Gprog SocketSpecs MonadExports
+     Representation AppLogic process_spec.
+
+From DeepWeb.Lib
+     Require Import VstLib.
+
+From DeepWeb.Proofs.Vst
+     Require Import VerifLib Connection SocketTactics.
+
+Import SockAPIPred.
+Import TracePred.
+
+Open Scope list.
+Open Scope logic.
+
+Opaque bind.
+
+Set Bullet Behavior "Strict Subproofs".
+
+Lemma body_process:
+  semax_body Vprog Gprog f_process (process_spec unit BUFFER_SIZE).
+Proof.
+  start_function.
+
+  assert_PROP (field_compatible (Tstruct _connection noattr)
+                                [] (conn_ptr))
+    by entailer!.
+
+  unfold rep_connection.
+  rewrite connection_list_cell_eq; [| assumption].
+
+  Intros.
+  forward.
+
+  forward_if.
+  {
+    unfold process_conn.
+    match goal with
+    | [H: Int.repr _ = Int.repr _ |- _] =>
+      destruct (conn_state conn) eqn:cstate;
+        try inversion H
+    end.
+
+    forward_call (k, st, conn, fd, last_msg, conn_ptr, msg_store_ptr).
+    {
+      unfold rep_connection.
+      rewrite connection_list_cell_eq; [| assumption].
+      rewrite cstate.
+      cancel.
+    }
+
+    Intro vret.
+    destruct vret as [[[conn' last_msg'] st'] ?].
+    simpl.
+
+    forward.
+    
+    Exists conn'.
+    Exists last_msg'.
+    Exists st'.
+    Exists YES.
+    
+    entailer!.
+    discriminate.
+    
+  }
+
+  forward_if.
+  {
+    unfold process_conn.
+    match goal with
+    | [H: Int.repr _ = Int.repr _ |- _] =>
+      destruct (conn_state conn) eqn:cstate;
+        try inversion H
+    end.
+
+    rewrite trace_bind_assoc.
+    
+    forward_call ( (fun conn => b <- ret (conn, last_msg) ;; k b),
+                   st, conn, fd, conn_ptr).
+    {
+      unfold rep_connection.
+      rewrite connection_list_cell_eq; [| assumption].
+      rewrite cstate.
+      cancel.
+
+      (* move to tactic *)
+      match goal with
+      | [|- context[ITREE ?tr1 * _ |-- ITREE ?tr2 * _]] =>
+        replace tr1 with tr2 by reflexivity
+      end.
+
+      cancel.
+
+    }
+
+    Intro vret.
+    destruct vret as [[conn' st'] ?].
+    simpl.
+
+    trace_bind_ret.
+
+    forward.
+    
+    Exists conn'.
+    Exists last_msg.
+    Exists st'.
+    Exists YES.
+    entailer!.
+    discriminate.
+    
+  }
+
+  unfold process_conn.
+
+  do 2 int_ineq_to_Z_ineq.
+
+  assert (conn_state conn = DELETED \/ conn_state conn = DONE) as cases by
+      (destruct (conn_state conn); try omega; auto).
+
+  forward.
+  
+  Exists conn.
+  Exists last_msg.
+  Exists st.
+  Exists YES.
+
+  repeat apply andp_right; auto.
+  - apply prop_right; repeat split; auto.
+    + intros Hstate; destruct cases; rewrite Hstate in *; discriminate.
+    + match goal with
+      | [H: _ = SENDING |- _] =>
+        rewrite H in *; destruct cases; discriminate
+      end.
+  - destruct cases as [Hstate | Hstate]; rewrite Hstate; 
+      trace_bind_ret;
+      unfold rep_connection;
+      rewrite connection_list_cell_eq; auto;
+        cancel.
+    all: rewrite Hstate; cancel.
+
+Qed.
