dw/DeepWeb/Proofs/Vst/verif_process_connections.v
@@ -1,0 +1,934 @@
+Require Import String.
+
+Require Import DeepWeb.Free.Monad.Verif.
+Require Import DeepWeb.Spec.Swap_CLikeSpec.
+
+From Custom Require Import List.
+
+From DeepWeb.Spec.Vst
+     Require Import MainInit Gprog SocketSpecs MonadExports
+     Representation AppLogic process_connections_spec.
+
+From DeepWeb.Lib
+     Require Import VstLib.
+
+From DeepWeb.Proofs.Vst
+     Require Import VerifLib SocketTactics 
+     Connection Store AppLib.
+
+Import SockAPIPred.
+Import TracePred.
+Import FDSetPred.
+
+Open Scope list.
+Open Scope logic.
+
+Set Bullet Behavior "Strict Subproofs".
+
+Opaque bind.
+
+Lemma proj_RECVING_SENDING: forall (c : connection * sockfd * val),
+    (has_conn_state RECVING c || has_conn_state SENDING c)%bool = true <->
+    (has_conn_state RECVING (proj_conn c)
+     || has_conn_state SENDING (proj_conn c))%bool = true.
+Proof.
+  intros [[c ?] ?].
+  simpl.
+  split;
+    intros H; apply orb_true_elim in H;
+      apply orb_true_intro;
+      destruct H; auto.
+Qed.        
+
+Definition process_loop_prop_invar
+           (connections : list (connection * sockfd * val))
+           (server_addr : endpoint_id)
+           (server_fd : sockfd)
+           (prefix suffix : list (connection * sockfd * val))
+           (st : SocketMap) :=
+  [consistent_world st;
+     Forall (fun '(conn, fd, ptr) =>
+               consistent_state BUFFER_SIZE st (conn, fd)) prefix;
+     Forall (fun '(conn, fd, ptr) =>
+               consistent_state BUFFER_SIZE st (conn, fd)) suffix;
+     exists old_prefix,
+     (connections = old_prefix ++ suffix /\
+      map proj_fd old_prefix = map proj_fd prefix /\
+      map conn_id
+          (map proj_conn old_prefix) = map conn_id (map proj_conn prefix) /\
+      map proj_ptr old_prefix = map proj_ptr prefix
+     );
+     
+     NoDup
+       (map conn_id
+            (map proj_conn
+                 (filter
+                    (fun c => (has_conn_state RECVING c
+                            || has_conn_state SENDING c)%bool)
+                    (prefix ++ suffix))));
+     
+     lookup_socket st server_fd = ListeningSocket server_addr].
+
+Definition process_loop_sep_invar
+           (k : SocketMonad unit)
+           (server_addr : endpoint_id)
+           (read_set : FD_Set)
+           (write_set : FD_Set)
+           (head_ptr : val)
+           (read_set_ptr : val)
+           (write_set_ptr : val)
+           (msg_store_ptr : val)
+           (prefix suffix: list (connection * sockfd * val))
+           (st : SocketMap)
+           (last_msg : string)
+           (curr_ptr : val)
+  :=
+    [SOCKAPI st ;
+     ITREE ( (select_loop
+                server_addr
+                BUFFER_SIZE
+                (true, (map proj_conn (prefix ++ suffix), last_msg)))
+               ;; k );
+     FD_SET Tsh read_set read_set_ptr;
+     FD_SET Tsh write_set write_set_ptr;
+     lseg LS Tsh Tsh (map rep_full_conn prefix) head_ptr curr_ptr;
+     lseg LS Tsh Tsh (map rep_full_conn suffix) curr_ptr nullval;
+     field_at Tsh (Tstruct _store noattr) [] (rep_store last_msg)
+              msg_store_ptr].
+
+Definition process_loop_invar
+           (k : SocketMonad unit)
+           (server_addr : endpoint_id)
+           (server_fd : sockfd)
+           (read_set : FD_Set)
+           (write_set : FD_Set)
+           (connections: list (connection * sockfd * val))
+           (head_ptr : val)
+           (read_set_ptr : val)
+           (write_set_ptr : val)
+           (msg_store_ptr : val)
+  : environ -> mpred :=
+  EX prefix : list (connection * sockfd * val),
+  EX suffix : list (connection * sockfd * val),
+  EX st : SocketMap,
+  EX last_msg : string,
+  EX curr_ptr : val,
+  PROPx (process_loop_prop_invar
+          connections server_addr server_fd prefix suffix st)
+  (LOCAL (
+      temp _head head_ptr;
+      temp _curr curr_ptr;
+      temp _rs read_set_ptr;
+      temp _ws write_set_ptr;
+      temp _last_msg_store msg_store_ptr
+     )
+  (SEPx (process_loop_sep_invar
+           k server_addr read_set write_set
+           head_ptr read_set_ptr write_set_ptr
+           msg_store_ptr prefix suffix st last_msg curr_ptr
+  ))).
+
+Definition process_loop_postcond
+           (k : SocketMonad unit)
+           (server_addr : endpoint_id)
+           (server_fd : sockfd)
+           (read_set : FD_Set)
+           (write_set : FD_Set)
+           (connections: list (connection * sockfd * val))
+           (head_ptr : val)
+           (read_set_ptr : val)
+           (write_set_ptr : val)
+           (msg_store_ptr : val)
+  : environ -> mpred :=
+  EX prefix : list (connection * sockfd * val),
+  EX suffix : list (connection * sockfd * val),
+  EX st : SocketMap,
+  EX last_msg : string,
+  EX curr_ptr : val,
+  PROPx ((curr_ptr = nullval)
+           ::  (process_loop_prop_invar
+                  connections server_addr server_fd prefix suffix st))
+  (LOCAL (
+      temp _head head_ptr;
+      temp _curr curr_ptr;
+      temp _rs read_set_ptr;
+      temp _ws write_set_ptr;
+      temp _last_msg_store msg_store_ptr
+     )
+  (SEPx (process_loop_sep_invar
+           k server_addr read_set write_set
+           head_ptr read_set_ptr write_set_ptr
+           msg_store_ptr prefix suffix st last_msg curr_ptr
+  ))).           
+
+
+Lemma body_process_connections:
+  semax_body Vprog Gprog f_process_connections
+             (process_connections_spec BUFFER_SIZE).
+Proof.
+  start_function.
+  
+  forward.
+
+  assert (forall conn fd ptr,
+             In (conn, fd, ptr) connections ->
+             descriptor server_fd <> descriptor fd) as all_fds_not_server_fd.
+  { 
+    intros conn fd ptr HIn.
+    unfold not.
+    intros fd_eq.
+    apply is_fd_irrelevant in fd_eq.
+    rewrite fd_eq in *.
+    
+    match goal with
+    | [H: Forall _ connections |- _] =>
+      rewrite Forall_forall in H;
+        specialize (H (conn, fd, ptr) HIn);
+        simpl in H;
+        apply consistent_connection_not_listening
+          with (addr := server_addr) in H
+    end.
+    tauto.
+
+  } 
+
+  set (inv := process_loop_invar k server_addr server_fd read_set write_set
+                                 connections conn_ptr
+                                 read_set_ptr write_set_ptr
+                                 msg_store_ptr).
+  set (postcond :=
+         process_loop_postcond k server_addr server_fd read_set write_set
+                               connections conn_ptr
+                               read_set_ptr write_set_ptr
+                               msg_store_ptr).
+
+  unfold Swhile.
+  forward_loop inv break:postcond.
+
+  { (* precondition *)
+
+    unfold process_loop_invar.
+    Exists ([] : list (connection * sockfd * val)).
+    Exists connections.
+    Exists st.
+    Exists last_msg.
+    Exists conn_ptr.
+
+    entailer!.
+
+    exists ([] : list (connection * sockfd * val)).
+    auto.
+
+  }
+  
+  { (* body of while *)
+
+    unfold inv, process_loop_invar.
+    Intros prefix.
+    Intros suffix.
+    Intros st0.
+    Intros last_msg0.
+    Intros curr_ptr.
+
+    focus_SEP 5; simpl.
+    unfold process_loop_prop_invar.
+
+    forward_if.
+    {
+      prove_lseg_ptr_null_test.
+    }
+
+    rewrite lseg_unfold.
+    destruct suffix as [| [[conn fd] ptr] rest].
+    { 
+      simpl.
+      Intros; tauto.
+    }
+
+    simpl.
+    Intros tail.
+    subst curr_ptr.
+
+    assert_PROP (field_compatible (Tstruct _connection noattr) []
+                                  ptr)
+      by entailer!.
+
+    assert (consistent_state BUFFER_SIZE st0 (conn, fd)) as Hconsistent.
+    { 
+      match goal with
+      | [H: Forall _  ((conn, fd, ptr) :: rest) |- _] =>
+        apply Forall_inv in H
+      end; assumption.
+    } 
+
+    focus_SEP 1.
+
+    unfold rep_connection.
+    rewrite connection_list_cell_eq; [| assumption].
+
+    Intros.
+
+    forward.
+
+    forward_call (fd, read_set, read_set_ptr, Tsh).
+    { split; auto.
+      eapply consistent_connection_fd_bound; eassumption.
+    }
+
+    Intro read_ready.
+
+    forward_call (fd, write_set, write_set_ptr, Tsh).
+    { split; auto.
+      eapply consistent_connection_fd_bound; eassumption.
+    }
+
+    Intro write_ready.
+
+    Intros.
+
+    forward.
+
+    (* FIXME: Freeze takes too long:
+       freeze [0; 1; 2; 3; 4; 5; 6; 7; 8; 9; 10; 11; 12; 13; 14; 15] FR1; 
+       simpl. *)
+
+    Local Ltac post_socket_ready read_ready write_ready :=
+      match goal with
+      | [|- context[LOCALx (_ :: ?locs) (SEPx ?sep)]] =>
+        forward_if
+          (EX socket_ready : Z,
+           PROP (socket_ready = 0 \/ socket_ready = 1;
+                 socket_ready = 1 -> read_ready <> 0 \/ write_ready <> 0)
+           (LOCALx (temp _socket_ready (Vint (Int.repr socket_ready)) :: locs)
+           (SEPx sep)))
+      end.
+    
+    post_socket_ready read_ready write_ready.
+    
+    { (* if read_ready *)
+      
+      forward.
+      Exists 1.
+
+      go_lower.
+      repeat apply andp_right; auto.
+      - apply prop_right; repeat split; auto. 
+      - apply prop_right; repeat split; auto.
+    }
+
+    (* else if write_ready *)
+    post_socket_ready read_ready write_ready.
+    
+    {
+      (* if write_ready *)
+      forward.
+      Exists 1.
+
+      go_lower.
+      repeat apply andp_right; auto.
+      - apply prop_right; repeat split; auto. 
+      - apply prop_right; repeat split; auto.
+        
+    }
+
+    { (* else *)
+      forward.
+      Exists 0.
+
+      go_lower.
+      repeat apply andp_right; auto.
+      - apply prop_right; repeat split; auto.
+        intros; omega.
+      - apply prop_right; repeat split; auto.
+
+    }
+
+    Intro socket_ready.
+    Intros.
+
+    gather_SEP 2 3 4 5 6 7 8.
+    repeat rewrite <- sepcon_assoc.
+    rewrite <- connection_list_cell_eq; [| assumption].
+    fold_rep_connection conn fd.
+    { 
+      unfold rep_connection.
+      go_lower.
+      cancel.
+    }
+
+    freeze [1; 2; 3; 4; 5; 8] FR1; simpl.
+    
+    set (tr conn last_msg :=
+           select_loop
+             server_addr
+             BUFFER_SIZE
+             (true, (map proj_conn
+                         (prefix ++ conn :: rest), last_msg))
+             ;; k).
+
+    (* process if ready *)
+
+    gather_SEP 1 2 3 4.
+    
+    Local Ltac post_process prefix suffix tr :=
+    match goal with
+    | [H: lookup_socket _ ?server_fd = ListeningSocket ?server_addr
+       |- context[LOCALx (?locs) (SEPx (?process_pred :: ?seps)) ]] =>
+    match process_pred with 
+    | context[list_cell _ _ (rep_connection ?conn ?fd) ?ptr] =>
+    match process_pred with 
+    | context[SOCKAPI ?st] => 
+    match process_pred with 
+    | context[field_at _ (Tstruct _store noattr) _
+                       (rep_store ?last_msg) ?msg_store_ptr] => 
+      forward_if
+      (EX conn' : connection,
+       EX last_msg' : string,              
+       EX st' : SocketMap,
+       PROP ( 
+           consistent_world st';
+           consistent_state BUFFER_SIZE st' (conn', fd);
+           Forall (fun '(conn, fd, _) =>
+                     consistent_state BUFFER_SIZE st' (conn, fd)) prefix;
+           Forall (fun '(conn, fd, _) =>
+                     consistent_state BUFFER_SIZE st' (conn, fd)) suffix;
+           lookup_socket st' server_fd = ListeningSocket server_addr;
+           conn_id conn = conn_id conn';
+           NoDup
+             (map conn_id
+                  (map proj_conn
+                       (filter
+                          (fun c : connection * sockfd * val =>
+                             (has_conn_state RECVING c
+                              || has_conn_state SENDING c)%bool)
+                          (prefix ++ (conn', fd, ptr) :: suffix))))
+         )
+       (LOCALx locs
+       (SEPx ( SOCKAPI st' ::
+               ITREE (tr (conn', fd, ptr) last_msg') ::
+               list_cell LS Tsh (rep_connection conn' fd) ptr ::
+               field_at Tsh (Tstruct _store noattr) []
+                        (rep_store last_msg') msg_store_ptr ::
+               seps )
+      )))
+    end
+    end
+    end
+    end.
+
+    post_process prefix rest tr.
+
+    { (* if (socket_ready > 0) *)
+
+      Intros.
+
+      unfold select_loop.
+      rewrite while_loop_unfold.
+      simpl.
+      rewrite trace_bind_assoc.
+      take_branch2 2.
+      rewrite trace_bind_assoc.
+
+      assert (socket_ready = 1) by omega.
+
+      match goal with
+      | [H1 : socket_ready = 1, H2 : socket_ready = 1 -> _ |- _] =>
+        pose proof (H2 H1); clear H1 H2
+      end.
+      
+      match goal with
+      | [H: exists old_prefix, _ |- _] =>
+        destruct H
+          as [old_prefix
+                [connections_eq
+                   [fds_preserved
+                      [ptrs_preserved ids_preserved]]]]
+      end.
+
+      rewrite connections_eq in *.
+
+      assert (In (descriptor fd) (map descriptor read_set)
+              \/ In (descriptor fd) (map descriptor write_set))
+        as fd_in_read_or_write.
+      { 
+        match goal with
+        | [H: read_ready <> 0 \/ _ |- _] =>
+          destruct H as [Hready | Hready]
+        end;
+          match goal with
+          | [H1 : read_ready <> 0 -> _,
+             H2 : write_ready <> 0 -> _ |- _] =>
+            try pose proof (H1 Hready) as in_set;
+              try pose proof (H2 Hready) as in_set
+          end.
+        - left; assumption.
+        - right; assumption.
+          
+      }
+
+      set (waiting_to_recv :=
+             map proj_fd
+                 (filter (has_conn_state RECVING)
+                         (old_prefix ++ (conn, fd, ptr) :: rest))).
+      
+      set (waiting_to_send :=
+             map proj_fd
+                 (filter (has_conn_state SENDING)
+                         (old_prefix ++ (conn, fd, ptr) :: rest))).
+      
+      assert (In (conn, fd, ptr) (old_prefix ++ (conn, fd, ptr) :: rest))
+        as conn_in.
+      {
+        apply in_or_app.
+        right.
+        simpl.
+        left; auto.
+      }
+
+      assert
+        (In (descriptor fd) (map descriptor waiting_to_recv)
+         \/ In (descriptor fd) (map descriptor waiting_to_send))
+        as fd_in_filtered.
+      { 
+        destruct fd_in_read_or_write
+          as [fd_in_read | fd_in_write]; [left | right];
+          match goal with
+          | [H1: context[fd_subset read_set _],
+             H2: context[fd_subset write_set _] |- _] =>
+            unfold fd_subset, incl in H1, H2;
+              try pose proof (H1 _ fd_in_read) as fd_in_recving;
+              try apply (H2 _ fd_in_write)
+          end.
+
+        specialize (all_fds_not_server_fd conn fd ptr conn_in).
+        simpl in fd_in_recving.
+        destruct fd_in_recving as [fd_eq |]; auto.
+        rewrite fd_eq in *; tauto.
+
+      }
+
+      assert (has_conn_state RECVING conn = true
+              \/ has_conn_state SENDING conn = true)
+        as conn_recving_sending.
+      {
+        destruct fd_in_filtered; [left | right];
+          eapply fd_in_filtered_implies_conn_state;
+          eauto.
+      }
+
+      match goal with
+      | [|- context[choose ?l]] =>
+        remember l as filtered_conns
+      end.
+
+      assert (In conn filtered_conns).
+      {
+
+        assert (In conn (map proj_conn (prefix ++ (conn, fd, ptr) :: rest))).
+        {
+          rewrite map_app.
+          simpl.
+          apply in_or_app.
+          right.
+          simpl.
+          left; auto.
+        }
+        
+        destruct conn_recving_sending; subst; apply in_or_app;
+          [left | right]; rewrite filter_In; split; auto.
+        
+      }
+
+      (* Choose conn in interaction tree. *)
+      rem_trace_tail process_tr.
+      replace_SEP 2 (ITREE (process_tr conn)).
+      {
+        go_lower.
+        apply internal_nondet3.
+        assumption.
+      }
+
+      subst process_tr.
+
+      rewrite trace_bind_assoc.
+
+      rem_trace_tail after_process.
+      forward_call (after_process, st0, conn, fd,
+                    last_msg0, ptr, msg_store_ptr).
+      { unify_trace.
+        cancel.
+      }
+      
+      (* after process *)
+      
+      Intro vret.
+      subst after_process.
+      destruct vret as [[[conn' last_msg'] st'] process_ret].
+      simpl fst; simpl snd.
+      Intros.
+      
+      assert (conn_state conn = RECVING \/ conn_state conn = SENDING)
+        as conn_RECVING_or_SENDING.
+      {
+        destruct conn_recving_sending as [Hconn_st | Hconn_st];
+          [left | right];
+          unfold has_conn_state in Hconn_st;
+          destruct QuickChick.Decidability.dec; try discriminate; auto.
+      }
+
+            
+      Local Ltac elim_conn_state conn :=
+        let Hconn_state := fresh "Hconn_state" in
+        match goal with
+        | [H: conn_state conn = _ \/ _ |- _] =>
+          destruct H as [ Hconn_state | Hconn_state ]
+        end;
+        match goal with
+        | [H1: conn_state conn = RECVING -> _,
+               H2: conn_state conn = SENDING -> _ |- _] =>
+          try (pose proof (H1 Hconn_state) as Hstep);
+          try (pose proof (H2 Hconn_state) as [Hstep last_msg'_eq])
+        end.        
+
+      assert
+        (Forall (fun '(conn0, fd0, _) =>
+                   consistent_state BUFFER_SIZE st' (conn0, fd0)) prefix
+         /\ Forall (fun '(conn0, fd0, _) =>
+                     consistent_state BUFFER_SIZE st' (conn0, fd0)) rest)
+        as frame_consistent.
+      {
+
+        elim_conn_state conn.
+        - eapply recv_step_preserves_frame_consistency
+            with (prefix := prefix) (suffix := rest); eauto.
+          Unshelve.
+          3 : { exact nullval. (* Irrelevant. *) } 
+          + match goal with
+            | [H: Forall _ (_ :: rest) |- _] =>
+              apply Forall_skipn with (n := 1%nat) in H; simpl in H
+            end.
+            assumption.
+          + repeat rewrite map_app in *.
+            rewrite <- fds_preserved.
+            auto.
+            
+        - eapply send_step_preserves_frame_consistency
+            with (prefix := prefix) (suffix := rest); eauto.
+          Unshelve.
+          3 : { exact nullval. (* Irrelevant. *) } 
+          + match goal with
+            | [H: Forall _ (_ :: rest) |- _] =>
+              apply Forall_skipn with (n := 1%nat) in H; simpl in H
+            end.
+            assumption.
+          + repeat rewrite map_app in *.
+            rewrite <- fds_preserved.
+            auto.
+            
+      } 
+
+      assert (conn_id conn = conn_id conn') as conn_id_preserved.
+      {
+        destruct conn_RECVING_or_SENDING as [ Hconn_state | Hconn_state ];
+          match goal with
+          | [H1: conn_state conn = RECVING -> _,
+                 H2: conn_state conn = SENDING -> _ |- _] =>
+            try (pose proof (H1 Hconn_state) as Hstep);
+              try (pose proof (H2 Hconn_state) as [Hstep last_msg'_eq])
+          end.
+        
+        - eapply recv_step_preserves_conn_ids; eauto.
+        - eapply send_step_preserves_conn_ids; eauto.
+      } 
+      
+      Exists conn'.
+      Exists last_msg'.
+      Exists st'.
+
+      entailer!.
+      
+      {
+        elim_conn_state conn.
+
+        (* RECVING *)
+        - repeat split; auto.
+          + eapply recv_step_preserves_consistency; eauto.
+          + destruct frame_consistent; auto.
+          + destruct frame_consistent; auto.
+          + match goal with
+            | [H: lookup_socket _ _ = _ |- _] =>
+              rewrite <- H
+            end.
+            symmetry.
+            eapply recv_step_preserves_frame_lookup; eauto.
+          + (* NoDup conn_ids preserved *)
+            match goal with
+            | [H: NoDup (map _ (map _ (filter _ (prefix ++ _ :: _)))) |- _] =>
+              revert H
+            end.
+            
+            repeat rewrite filter_app; repeat rewrite map_app.
+            simpl.
+
+            replace ((has_conn_state _ _ || _)%bool) with true
+              by (symmetry; apply orb_true_intro; auto).
+
+            simpl.
+            destruct ((has_conn_state _ _ || _)%bool);
+              try (simpl; rewrite conn_id_preserved;
+                   intros; assumption);
+              try (intros HNoDup;
+                   eapply NoDup_remove_1; eassumption).
+            
+        - (* SENDING *)
+          repeat split; auto.
+          + eapply send_step_preserves_consistency; eauto.
+          + destruct frame_consistent; auto.
+          + destruct frame_consistent; auto.
+          + match goal with
+            | [H: lookup_socket _ _ = _ |- _] =>
+              rewrite <- H
+            end.
+            symmetry.
+            eapply send_step_preserves_frame_lookup; eauto.
+          + (* NoDup conn_ids preserved *)
+            match goal with
+            | [H: NoDup (map _ (map _ (filter _ (prefix ++ _ :: _)))) |- _] =>
+              revert H
+            end.
+            
+            repeat rewrite filter_app; repeat rewrite map_app.
+            simpl.
+
+            replace ((has_conn_state _ _ || _)%bool) with true
+              by (symmetry; apply orb_true_intro; auto).
+
+            simpl.
+            destruct ((has_conn_state _ _ || _)%bool);
+              try (simpl; rewrite conn_id_preserved;
+                   intros; assumption);
+              try (intros HNoDup;
+                   eapply NoDup_remove_1; eassumption).
+            
+      } 
+
+      trace_bind_ret.  
+      subst tr.
+      unfold select_loop.
+      replace
+        (replace_when _ conn' _)
+        with 
+          (map proj_conn (prefix ++ (conn', fd, ptr) :: rest));
+        [cancel |].
+      
+      repeat rewrite map_app.
+      simpl.
+
+      rewrite replace_when_NoDup
+        with (g := conn_id)
+             (p2 := (fun c => has_conn_state RECVING c
+                           || has_conn_state SENDING c)%bool)
+             (n := conn_id conn'); auto.
+      
+      - (* discriminator *)
+        intros.
+        rewrite conditional_bool.
+        rewrite conditional_dec_true.
+        reflexivity.
+        
+      - (* conn_id the same and matches filter condition *)
+        split; auto.
+        apply orb_true_intro.
+        destruct conn_RECVING_or_SENDING; [left | right];
+          unfold has_conn_state;
+          destruct (QuickChick.Decidability.dec);
+          auto;
+          tauto.
+
+      - rewrite filter_app.
+        rewrite map_app.
+        apply NoDup_remove_2.
+
+        match goal with
+        | [H: NoDup
+                (map _ (map _ (filter _ (prefix ++ (conn, fd, ptr) :: rest))))
+           |- _] =>
+          revert H
+        end.
+        
+        rewrite filter_app.
+        rewrite map_app.
+        simpl.
+
+        assert (has_conn_state RECVING (conn, fd, ptr) = true
+                \/ has_conn_state SENDING (conn, fd, ptr) = true) as cond_true.
+        { 
+          destruct conn_RECVING_or_SENDING;
+            [left | right];
+            unfold has_conn_state;
+            destruct (QuickChick.Decidability.dec);
+            auto;
+            tauto.
+        }
+
+        apply orb_true_intro in cond_true.
+        rewrite cond_true.
+        rewrite map_app.
+        simpl.
+
+        do 2 rewrite filter_proj_commutes
+          with (p2 := fun c : connection =>
+                        (has_conn_state RECVING c || has_conn_state SENDING c)%bool)
+          by (apply proj_RECVING_SENDING).          
+
+        intros; assumption.
+
+    } (* end if (socket_ready > 0) { process; } *)
+
+
+    { (* else *)
+
+      forward.
+      Exists conn.
+      Exists last_msg0.
+      Exists st0.
+
+      go_lower.
+      repeat apply andp_right; auto.
+      - apply prop_right; repeat split; auto.
+        (* prefix still consistent *)
+        match goal with
+        | [H: Forall _ ((conn, fd, ptr) :: rest) |- _] => 
+          apply (Forall_skipn _ _ 1%nat) in H;
+            simpl in H
+        end.
+        assumption.
+      - apply prop_right; repeat split; auto.
+      - subst tr.
+        cancel.
+
+    }
+
+    Intro conn'.
+    Intro last_msg'.
+    Intro st'.
+    Intros.
+
+    match goal with
+    | [H: exists old_prefix, _ |- _] =>
+      destruct H
+        as [old_prefix
+              [connections_eq
+                 [fds_preserved
+                    [ids_preserved ptrs_preserved]]]]
+    end.
+
+    thaw FR1; simpl.
+
+    forward.    
+
+    gather_SEP 2 7 8.
+    Intros.
+    gather_SEP 0 8 2 1.
+    fold_conn_cell_into_prefix.
+    Intros.    
+
+    unfold inv, process_loop_invar.
+
+    Exists (prefix ++ [(conn', fd, ptr)]) .
+    Exists rest.
+    Exists st'.
+    Exists last_msg'.
+    Exists tail.
+        
+    go_lower.
+    repeat apply andp_right; auto.
+    
+    - apply prop_right; repeat split; auto.
+      + (* Consistency of prefix *)
+        rewrite Forall_app; split; auto.
+
+      + (* Extend old prefix *)
+        exists (old_prefix ++ [(conn, fd, ptr)]).
+        repeat split; [ rewrite <- app_assoc; auto | ..].
+        * repeat rewrite map_app; simpl.
+          rewrite fds_preserved.
+          reflexivity.
+        * repeat rewrite map_app; simpl.
+          rewrite ids_preserved.
+          replace (conn_id conn) with (conn_id conn') by assumption.
+          reflexivity.
+        * repeat rewrite map_app; simpl.
+          rewrite ptrs_preserved.
+          reflexivity.
+      + (* NoDup conn_ids *)
+        rewrite <- app_assoc.
+        simpl.
+        assumption.
+    - apply prop_right; repeat split; auto.
+      
+    - cancel.
+      subst tr.
+      simpl.
+      repeat rewrite <- app_assoc; simpl.
+      cancel.
+      rewrite map_app.
+      simpl.
+      cancel.
+
+    - (* break *)
+      forward.
+      subst postcond; unfold process_loop_postcond.
+      Exists prefix.
+      Exists suffix.
+      Exists st0.
+      Exists last_msg0.
+      Exists curr_ptr.
+      entailer!.
+      
+  }
+  
+  (* Exit from loop *)
+
+  subst postcond.
+  unfold process_loop_postcond.
+
+  Intros prefix.
+  Intros suffix.
+  Intros st'.
+  Intros last_msg'.
+  Intros curr_ptr.
+  unfold process_loop_prop_invar, process_loop_sep_invar.
+  
+  subst curr_ptr.
+  rewrite lseg_eq; auto.
+  Intros.
+  assert (suffix = []) by (eapply map_eq_nil; eassumption).
+  subst suffix.
+  rewrite app_nil_r.
+  
+  match goal with
+  | [H: exists old_prefix, _ |- _] =>
+    destruct H
+      as [connections'
+            [connections_eq
+               [fds_preserved
+                  [ids_preserved ptrs_preserved]]]];
+      rewrite app_nil_r in connections_eq;
+      subst connections'
+  end.
+
+  match goal with
+  | [H: NoDup (map _ (map _ (filter _ (prefix ++ [])))) |- _] =>
+    rewrite app_nil_r in H
+  end.
+  
+  forward.
+
+  Exists prefix.
+  Exists last_msg'.
+  Exists st'.
+
+  entailer!.
+  
+Qed.
