dw/DeepWeb/Proofs/Vst/verif_prog.v
@@ -1,0 +1,229 @@
+Require Import DeepWeb.Spec.TopLevelSpec.
+Require Import DeepWeb.Spec.Swap_CLikeSpec.
+
+From DeepWeb.Spec.Vst
+     Require Import MainInit Gprog SocketSpecs
+     MonadExports LibrarySpecs
+     zeroize_addr_spec bind_socket_spec new_store_spec init_store_spec
+     new_connection_spec reset_connection_spec
+     populate_response_spec check_if_complete_spec
+     accept_connection_spec conn_read_spec conn_write_spec
+     process_spec add_to_fd_set_spec
+     monitor_connections_spec process_connections_spec
+     select_loop_spec.
+
+From DeepWeb.Proofs.Vst
+     Require Import verif_main verif_bind_socket verif_new_store
+     verif_init_store verif_new_connection verif_reset_connection
+     verif_populate_response verif_check_if_complete
+     verif_accept_connection verif_conn_read verif_conn_write
+     verif_process verif_add_to_fd_set verif_monitor_connections
+     verif_process_connections verif_select_loop.
+
+Ltac rem_rest := 
+  match goal with
+  | |- semax_func _ _ (?hd1 :: ?tl1) (?hd2 :: ?tl2) =>
+    remember tl1 as rest1;
+    remember tl2 as rest2
+  end.
+
+Ltac unify_spec :=
+  match goal with
+  | [H: semax_body _ _ _ ?spec1 |- semax_body _ _ _ ?spec2] =>
+    replace spec2 with spec1;
+    [apply H |];
+    unfold NDmk_funspec;
+    try unfold spec1;
+    f_equal
+  end.
+
+Ltac extract_ret_val :=
+  match goal with
+  | [|- context[PROPx _ (LOCALx [temp _ _] _) ]] =>
+    let H := fresh "Hret" in
+    rewrite <- insert_local;
+    rewrite lower_andp;
+    apply derives_extract_prop; intros H;
+    hnf in H;
+    rewrite retval_ext_rval in H
+  end.
+
+Ltac lower_to_SEP :=
+  match goal with
+  | |- context[PROPx _ (LOCALx _ (SEPx ?sep)) ?rho |-- ?rhs] =>
+    let H := fresh "Hlower" in
+    pose proof (finish_lower rho (fun _ => True) sep rhs) as H;
+    rewrite <- local_andp_lemma in H by (apply local_True_right);
+    apply H; clear H;
+    intros _; simpl
+  end.
+
+Ltac semax_func_cons' L :=
+  apply semax_func_cons;
+  [ subst; auto 
+  | repeat apply Forall_cons; try apply Forall_nil; computable
+  | unfold var_sizes_ok; repeat constructor
+  | reflexivity
+  | precondition_closed
+  | let H := fresh "body" in
+    pose proof L;
+    try solve [unify_spec]
+  | ].
+
+Lemma all_funcs_correct:
+  semax_func Vprog Gprog (prog_funct prog) Gprog.
+Proof.
+  unfold Gprog at 2. 
+  unfold prog, prog_funct; simpl.
+
+  repeat (apply semax_func_cons_ext_vacuous; [reflexivity | reflexivity | ]).
+
+  semax_func_cons body_malloc.
+  apply semax_func_cons_malloc_aux.
+
+  semax_func_cons_ext.
+
+  semax_func_cons_ext.
+
+  { (* typechecking for memcpy *)
+
+    extract_ret_val.
+    subst v.
+    lower_to_SEP.
+    entailer!.
+  } 
+  
+  semax_func_cons_ext.
+  { (* typechecking for memset *)
+
+    extract_ret_val.
+    subst v.
+    lower_to_SEP.
+    entailer!.
+  } 
+
+  semax_func_cons_ext.
+
+  semax_func_cons_ext.
+  semax_func_cons_ext.
+  semax_func_cons_ext.
+  semax_func_cons_ext.
+  semax_func_cons_ext.
+  semax_func_cons_ext.
+  semax_func_cons_ext.
+  semax_func_cons_ext.
+
+  { (* typechecking for htons *)
+    extract_ret_val.
+    rewrite <- Hret.
+
+    match goal with
+    | |- context[(PROPx (?prop :: ?other_prop) ?rest) ?rho |-- ?rhs] =>
+      apply (derives_extract_PROP' prop other_prop
+                                   rest (fun _ => rhs))
+    end.
+
+    intros bound.
+    simpl.
+    intros e.
+    entailer!.
+    omega.
+    
+  } 
+
+  (* select *)
+  semax_func_cons_ext.
+  
+  semax_func_cons' body_fd_zero_macro.
+  semax_func_cons' body_fd_isset_macro.
+  semax_func_cons' body_fd_set_macro.
+  semax_func_cons' body_check_if_complete.
+  { 
+    unfold check_if_complete_spec in H.
+    unify_spec.
+  } 
+
+  semax_func_cons' body_new_connection.
+
+  semax_func_cons' body_new_store.
+
+  semax_func_cons' body_populate_response.
+
+  semax_func_cons' body_conn_read.
+  { unfold conn_read_spec in H.
+    unify_spec.
+  } 
+    
+  semax_func_cons' body_reset_connection.
+
+  semax_func_cons' body_conn_write.
+  { 
+    unfold conn_write_spec in H.
+    unify_spec.
+  } 
+
+  semax_func_cons' body_process.
+  { 
+    unfold process_spec in H.
+    unify_spec.
+  } 
+
+  semax_func_cons' body_accept_connection.
+  { 
+    unfold accept_connection_spec in H.
+    unify_spec.
+  } 
+  
+  semax_func_cons' body_add_to_fd_set.
+
+  semax_func_cons' body_monitor_connections.
+
+  semax_func_cons' body_process_connections.
+  { 
+    unfold process_connections_spec in H.
+    unify_spec.
+  } 
+
+  apply semax_func_cons.
+  { subst; auto. }
+  { apply Forall_cons; auto.
+    apply Forall_cons; auto.
+  } 
+  { unfold var_sizes_ok.
+    repeat (apply Forall_cons; [simpl; rep_omega | ]).
+    constructor.
+  } 
+  { auto. }
+  { precondition_closed. } 
+  { pose proof body_select_loop.
+    unfold select_loop_spec in H.
+    unify_spec.
+  } 
+
+  semax_func_cons' body_zeroize_addr.
+
+  apply semax_func_cons.
+  { subst; auto. }
+  { apply Forall_cons; auto. } 
+  { repeat (apply Forall_cons; [simpl; rep_omega | ]).
+    constructor.
+  } 
+  { auto. }
+  { precondition_closed. } 
+  {
+    pose proof body_bind_socket.
+    unfold bind_socket_spec in H.
+    unify_spec.
+  }
+
+  semax_func_cons' body_init_store.
+
+  semax_func_cons' body_main.
+  {
+    unfold main_spec in H.
+    unify_spec.
+  }
+
+  apply semax_func_nil.
+  
+Qed.
