dw/DeepWeb/Spec/TopLevelSpec.v
@@ -1,0 +1,21 @@
+From DeepWeb Require Import
+     Lib.SimpleSpec
+     Lib.NetworkAdapter
+     Spec.Swap_SimpleSpec.
+
+From DeepWeb.Spec.Vst Require Import
+     MainInit
+     Gprog
+     SocketSpecs.
+
+Import TracePred.
+
+Definition swap_spec := swap_spec_ (Z.to_nat BUFFER_SIZE) INIT_MSG.
+
+(* *** The top-level correctness property.  (Proof of this is in 
+   Proofs/TopLevelProof.v) *)
+
+Definition swap_server_correct :=
+  exists (tree : SocketMonad unit),
+    refines_mod_network (simplify_network tree) swap_spec /\
+    semax_prog_ext prog tree Vprog Gprog.
