dw/DeepWeb/Spec/Vst/Gprog.v
@@ -1,0 +1,116 @@
+From VST
+     Require Import sepcomp.extspec veric.juicy_mem veric.semax_ext.
+
+Require Import DeepWeb.Spec.Swap_CLikeSpec.
+
+From DeepWeb.Spec.Vst
+     Require Import MainInit SocketSpecs
+     MonadExports LibrarySpecs
+     zeroize_addr_spec bind_socket_spec new_store_spec init_store_spec
+     new_connection_spec reset_connection_spec
+     populate_response_spec check_if_complete_spec
+     accept_connection_spec conn_read_spec conn_write_spec
+     process_spec add_to_fd_set_spec
+     monitor_connections_spec process_connections_spec
+     select_loop_spec.
+
+
+Import TracePred.
+Import SockAPIPred.
+
+Definition void_spec T : external_specification juicy_mem external_function T :=
+    Build_external_specification
+      juicy_mem external_function T
+      (fun ef => False)
+      (fun ef Hef ge tys vl m z => False)
+      (fun ef Hef ge ty vl m z => False)
+      (fun rv m z => False).
+
+Definition ok_void_spec (T : Type) : OracleKind.
+ refine (Build_OracleKind T (Build_juicy_ext_spec _ (void_spec T) _ _ _)).
+Proof.
+  simpl; intros; contradiction.
+  simpl; intros; contradiction.
+  simpl; intros; intros ? ? ? ?; contradiction.
+Defined.
+
+Definition ext_link := ext_link_prog main.prog.
+
+Definition socket_ext_spec
+  :=
+  add_funspecs_rec
+    ext_link
+    (ok_void_spec (SocketMonad unit)).(@OK_ty)
+    (ok_void_spec (SocketMonad unit)).(@OK_spec)
+    socket_specs.
+
+Instance Socket_Espec : OracleKind :=
+  Build_OracleKind
+    (SocketMonad unit)
+    (socket_ext_spec).
+
+Definition main_spec (tree : SocketMonad unit) :=
+  DECLARE _main
+  WITH gv : globals
+  PRE [ _argc OF tint, _argv OF (tptr (tptr tschar)) ]
+  (PROP ( )
+   LOCAL (gvars gv)
+   SEP (SOCKAPI {| lookup_socket := fun _ : sockfd => ClosedSocket |} ;
+        ITREE tree))
+  POST [ tint ]
+  PROP ( False )
+  LOCAL ( temp ret_temp (Vint (Int.repr 0)) )
+  SEP ( ).
+
+Definition Vprog : varspecs. mk_varspecs prog. Defined.
+
+(* Packaging the API spec all together. *)
+
+Definition specs :=
+  socket_specs
+    ++
+    [  memset_spec;
+       memcpy_spec;
+
+       fd_zero_macro_spec;
+       fd_set_macro_spec;
+       fd_isset_macro_spec;
+       htons_spec;
+
+       zeroize_addr_spec;
+       bind_socket_spec;
+       new_store_spec;
+       init_store_spec;
+       check_if_complete_spec BUFFER_SIZE;
+       populate_response_spec;  
+       new_connection_spec;
+       reset_connection_spec;
+       accept_connection_spec unit;
+       conn_read_spec unit BUFFER_SIZE;
+       conn_write_spec unit BUFFER_SIZE;
+       process_spec unit BUFFER_SIZE;
+       monitor_connections_spec;
+       process_connections_spec BUFFER_SIZE;
+       select_loop_spec;
+       add_to_fd_set_spec; 
+       
+       main_spec server
+    ].
+
+Definition Gprog : funspecs :=
+  ltac:(with_library prog specs).
+
+Instance Espec : OracleKind :=
+  add_funspecs Socket_Espec (ext_link_prog prog) Gprog.
+
+Axiom body_fd_zero_macro:
+  semax_body Vprog Gprog f_fd_zero_macro fd_zero_macro_spec.
+
+Axiom body_fd_set_macro:
+  semax_body Vprog Gprog f_fd_set_macro fd_set_macro_spec.
+
+Axiom body_fd_isset_macro:
+  semax_body Vprog Gprog f_fd_isset_macro fd_isset_macro_spec.
+
+Axiom body_zeroize_addr:
+  semax_body Vprog Gprog f_zeroize_addr zeroize_addr_spec.
