dw/DeepWeb/Spec/Vst/MonadExports.v
@@ -1,0 +1,7 @@
+Require Export DeepWeb.Free.Monad.Free.
+Require Export DeepWeb.Free.Monad.Common.
+Require Export DeepWeb.Free.Monad.Verif.
+
+Require Export Custom.Monad.
+Export MonadNotations.
+Open Scope monad_scope.
