dw/DeepWeb/Spec/Vst/bind_socket_spec.v
@@ -1,0 +1,31 @@
+Require Import String.
+
+Require Import DeepWeb.Lib.Util.
+Require Import DeepWeb.Lib.NetworkInterface.
+From DeepWeb.Spec
+     Require Import Vst.MainInit Vst.SocketSpecs.
+
+Import SockAPIPred.
+
+Definition bind_socket_spec :=
+  DECLARE _bind_socket
+  WITH st : SocketMap,
+       fd : sockfd,
+       addr : endpoint_id
+  PRE [ _fd OF tint, _port OF tint ] 
+    PROP ( consistent_world st ; 0 <= port_number addr <= two_p 16 - 1 )
+    LOCAL ( temp _fd (Vint (Int.repr (descriptor fd)));
+            temp _port (Vint (Int.repr (port_number addr)))
+          )
+    SEP ( SOCKAPI st )
+  POST [ tint ]
+    EX st' : SocketMap,
+    EX r : Z, 
+    PROP ( r = YES \/ r = NO ;
+             r = YES -> lookup_socket st fd = OpenedSocket /\
+                       st' = update_socket_state st fd (BoundSocket addr) ;
+             r = NO -> st' = st;
+             consistent_world st'
+         )
+    LOCAL ( temp ret_temp (Vint (Int.repr r)) )
+    SEP ( SOCKAPI st' ).
