dw/DeepWeb/Spec/Vst/new_connection_spec.v
@@ -1,0 +1,41 @@
+Require Import String.
+
+From DeepWeb.Spec
+     Require Import Vst.MainInit Vst.SocketSpecs Vst.Representation
+     Swap_CLikeSpec.
+
+Require Import DeepWeb.Lib.VstLib.
+
+Definition new_connection_spec :=
+  DECLARE _new_connection
+  WITH tt : unit
+  PRE [] 
+    PROP ()
+    LOCAL ()
+    SEP ()
+  POST [ (tptr (Tstruct _connection noattr)) ]
+    EX conn_opt : option connection,
+    EX r : val, 
+    PROP ( isptr r \/ r = nullval ;
+             isptr r ->
+             (conn_opt = Some {| conn_id := Connection 0%nat; (* dummy *)
+                                 conn_request := "";
+                                 conn_response := "";
+                                 conn_response_bytes_sent := 0;
+                                 conn_state := RECVING
+                              |})
+             ;
+             r = nullval -> conn_opt = None
+         )
+    LOCAL ( temp ret_temp r )
+    SEP (
+      let zero_fd := {| descriptor := 0; is_descriptor := zero_is_fd |} in
+      match conn_opt with
+      | Some conn =>
+        malloc_token Tsh (Tstruct _connection noattr) r *
+        lseg LS Tsh Tsh
+             ([(r, rep_connection conn zero_fd)])
+             r nullval
+      | None => emp
+      end
+    ).
