dw/DeepWeb/Spec/Vst/zeroize_addr_spec.v
@@ -1,0 +1,22 @@
+From DeepWeb.Spec
+     Require Import Vst.MainInit Vst.SocketSpecs.
+
+Import SockAddr.
+
+Definition zeroize_addr_spec :=
+  DECLARE _zeroize_addr
+  WITH ptr : val
+  PRE [ _addr OF tptr (Tstruct _sockaddr_in noattr) ]
+    PROP ( ) 
+    LOCAL ( temp _addr ptr )
+    SEP ( data_at_ Tsh (Tstruct _sockaddr_in noattr) ptr )
+  POST [ tvoid ]
+    PROP ( )
+    LOCAL ( )
+    SEP ( data_at Tsh (Tstruct _sockaddr_in noattr)
+                  (rep_sockaddr {| sin_family := 0;
+                                   sin_port := 0;
+                                   sin_addr := 0
+                                |})
+                  ptr
+        ).
